Proof of missing lemma in Local.v

theories/Local.v
@@ -633,11 +633,7 @@ Section Semantics.
     | _ => None
     end%fmap.
 
-    Definition run_act_lt (L : rl_ty) A :=
-      match do_act_lt L A with
-      | Some L' => L
-      | None => L
-      end.
+    Definition run_act_lt (L : rl_ty) A := odflt L (do_act_lt L A).
 
     Definition do_act (P : renv) A :=
       let: (mk_act a p q l t) := A in
@@ -803,8 +799,169 @@ Section Semantics.
       by apply/(CIH _ _ _ UG EG).
   Qed.
 
-  Lemma do_act_works : forall Li Lr A, LUnroll Li Lr -> LUnroll (run_act_l_ty Li A) (run_act_lt Lr A).
-  Admitted.
+  Fixpoint n_rec d L :=
+    match d with
+    | 0 => L
+    | d.+1 => l_rec (n_rec d L)
+    end.
+
+  Fixpoint n_open d n L :=
+    match n with
+    | 0 => L
+    | m.+1 => l_open d (n_rec d.+1 (n_open d.+1 m L)) (n_open d.+1 m L)
+    end.
+
+  Fixpoint get_nr L :=
+    match L with
+    | l_rec L => get_nr L
+    | _ => L
+    end.
+
+  Lemma nrec_comm d L : n_rec d (l_rec L) = n_rec d.+1 L.
+  Proof. by elim: d =>//= n ->. Qed.
+
+  Lemma nopen_rec_comm n L : n_open 0 n (l_rec L) = l_rec (n_open 1 n L).
+  Proof.
+    elim: n 0 L=>//= n Ih d L.
+    rewrite Ih/= -Ih/= -/(n_rec d.+1 _) -/(n_rec d.+2 _).
+    by rewrite Ih -/(n_rec d.+2 _) nrec_comm.
+  Qed.
+
+  Lemma lunroll_nopen L :
+    lunroll (lrec_depth L) L = n_open 0 (lrec_depth L) (get_nr L).
+  Proof.
+    rewrite -{2}/(n_open 0 0 L) -{2}(@addn0 (lrec_depth L)); move: {2 4}0 => n.
+    elim: L n=>//= L Ih n.
+    rewrite nopen_rec_comm/= -/(n_open 0 (lrec_depth L + n).+1 _).
+    by rewrite -/(n_open 0 n.+1 _); rewrite Ih addnS.
+  Qed.
+
+  Lemma nopen_end d : n_open 0 d l_end = l_end.
+  Proof. by elim: d 0 =>[|d Ih] n //=; rewrite Ih/=. Qed.
+
+  Lemma nopen_var m n L v : n_open m n L = l_var v -> L = l_var v.
+  Proof.
+    elim: n m=>//= n Ih m.
+    case EQ: n_open=>[|v'||]//=; case: ifP=>// _ [EV].
+    by move: EV EQ=>->{v'}/Ih.
+  Qed.
+
+  Lemma nopen_msg m n L a p C :
+    n_open m n L = l_msg a p C ->
+    exists C', L = l_msg a p C'.
+  Proof.
+    elim: n =>[| n Ih]//= in m C *;
+      first by move=>->; exists C; congr l_msg; elim: C=>//= [][l][Ty] G Ks<-.
+    case EQ: n_open=>[|v||a' p' C']//=; first by case: ifP.
+    move=> [EQa EQp EQc]; move: EQa EQp EQc EQ=>->-> EQc EQ{a' p'}.
+    by move: (Ih _ _ EQ).
+  Qed.
+
+  Lemma getnr_nonrec L : match get_nr L with
+                         | l_rec _ => false
+                         | _ => true
+                         end.
+  Proof. by elim: L. Qed.
+
+  Lemma nopen_rec d n L L' :
+    n_open d n (get_nr L) = l_rec L' ->
+    exists m, l_binds m (get_nr L) /\ m < d + n.
+  Proof.
+    elim: n =>[|n Ih] //= in d L' *;
+      first by move=> H; move: H (getnr_nonrec L)=>->.
+    case EQ: (n_open d.+1 n (get_nr L)) => [|v|Lr|]//=.
+    - case: ifP=>///eqP-EV; rewrite (nopen_var EQ)/=EV =>{}EQ.
+      exists d; rewrite eq_refl; split=>//.
+      rewrite addnS; by apply/leq_addr.
+    - move: (Ih _ _ EQ)=>[m][BND] LE _.
+      by exists m; split=>//; rewrite addnS.
+  Qed.
+
+  Lemma lopen_nrec d m L
+    : l_open d L (n_rec m (l_var m)) = n_rec m (if d == 0 then L else l_var m).
+  Proof.
+    rewrite -{2 4}(add0n m) -{1}(add0n d); move: {-3}0=>n.
+    elim: m=>[|m Ih]/= in n *.
+    - case: (ifP (d == 0))=>[/eqP->|]; first by rewrite eq_refl.
+      by case: ifP=>//; rewrite eqn_add2l eq_sym=>->.
+    - by rewrite addnS -!addSn Ih.
+  Qed.
+
+  Lemma nopen_var_rec d n m :
+    n_open d n (l_var m) = if (m < d) || (m >= d + n)
+                           then l_var m else n_rec m.+1 (l_var m).
+  Proof.
+    elim: n=>[|n Ih]/= in d *.
+    - by rewrite addn0 leqNgt orNb.
+    - rewrite Ih; case: (ifP ((m < d) || _ ))=>[/orP-[]|]H.
+      + move: H (leqW H); rewrite ltn_neqAle=>/andP-[/negPf-NE _]->/=.
+        by rewrite NE.
+      + move: H; rewrite addnS addSn => H; rewrite H orbC/=.
+        move: (leq_ltn_trans (leq_addr n d) H).
+        by rewrite ltn_neqAle eq_sym=>/andP-[/negPf-> _]/=.
+      + move: H=>/(rwP negPf); rewrite negb_or addnS addSn andbC=>/andP-[H1].
+        rewrite (negPf H1) orbF ltn_neqAle negb_and negbK=>/orP-[]H2.
+        * by move: H2 H1=>/eqP-<-{d} _; rewrite leqnn /= eq_refl.
+        * rewrite /leq/subn/=-/subn-/(leq m d) (negPf H2)/=; congr l_rec.
+          by rewrite lopen_nrec.
+  Qed.
+
+  Lemma getnr_nrec m v : get_nr (n_rec m (l_var v)) = l_var v.
+  Proof. by elim m. Qed.
+
+  Lemma lrecdepth_nrec m v : lrec_depth (n_rec m (l_var v)) = m.
+  Proof. by elim m=>//= n ->. Qed.
+
+  Lemma lunroll_inf Li Lr Li' :
+    lunroll (lrec_depth Li) Li = l_rec Li' ->
+    LUnroll Li Lr.
+  Proof.
+    rewrite lunroll_nopen=>/nopen_rec-[m]; rewrite add0n=>[][BND].
+    rewrite -(@add0n (lrec_depth _)) -{2}/(n_open 0 0 Li).
+    move: {-2}0=>n; move EQ: (n_open 0 n Li) => L mn.
+    move: {EQ BND mn} (conj EQ (conj BND mn))=> H.
+    move: (ex_intro (fun=>_) m H)=>{m}H.
+    move: (ex_intro (fun=>_) n H)=>{n}H.
+    move: (ex_intro (fun=>_) Li H)=>{Li Li'}H.
+    move: L Lr H; apply/paco2_acc=>r _.
+    move=>/(_ _ _ (ex_intro _ _ (ex_intro _ _ (ex_intro _ _ (conj erefl (conj _ _))))))-CIH.
+    move=> L Lr [Li][n][m][<-]{L}[BND][REC].
+    move: BND REC; case: Li=>//=.
+    - move=> v /eqP->; rewrite addn0=>mn/=.
+      rewrite nopen_var_rec ltn0 leqNgt mn /negb/orb=>{mn n v}.
+      move=>/=; apply/paco2_fold; constructor; right.
+      rewrite -/(n_open _ 1 _); apply/(CIH 1 _ _ m);
+        first by rewrite getnr_nrec/= eq_refl.
+      by rewrite lrecdepth_nrec.
+    - move=> L; rewrite nopen_rec_comm.
+      move=>BND LE; apply/paco2_fold; constructor.
+      rewrite -/(n_open _ n.+1 _); right; apply/(CIH _ _ _ _ BND).
+      by move: LE; rewrite addnS.
+  Qed.
+
+  Lemma do_act_works Li Lr A :
+    LUnroll Li Lr -> LUnroll (run_act_l_ty Li A) (run_act_lt Lr A).
+  Proof.
+    rewrite /run_act_l_ty/run_act_lt/do_act_l_ty/do_act_lt/==>LU.
+    case: A=> a _ q l t; move: ((LUnroll_ind (lrec_depth Li) Li Lr).1 LU)=>LU'.
+    move: LU' LU.
+    case EQ: (lunroll (lrec_depth Li) Li)=>
+    [
+    | v
+    | Li'
+    | a' p C
+    ].
+    - by move=> /lunroll_end->.
+    - by move=>/(paco2_unfold l_unroll_monotone); case F: _ _ /.
+    - by move=>/= _ _; apply/(lunroll_inf _ EQ).
+    - move=>/(paco2_unfold l_unroll_monotone).
+      case F: _ _ / =>[||a0 p0 K0 C0 DOM UNR]//.
+      move: F DOM UNR=>[<-<-<-] DOM UNR{a0 p0 K0 EQ}.
+      case EQ: find_cont=>[[Ty L]|]//; last by rewrite (dom_none DOM EQ).
+      move: (dom DOM EQ)=>[{}Lr] EQ'; rewrite EQ'/=.
+      case: (boolP ((a == a') && (q == p) && (t == Ty)))=>//= _ _.
+      by move: (UNR _ _ _ _ EQ EQ')=>[].
+  Qed.
 
   Open Scope fmap_scope.
   (** lstep a Q P Q' P' is the 'step' relation <P, Q> ->^a <P', Q'> in Coq*)
